theories/OGS/spec'.v
@@ -1,357 +1,56 @@
-  Context {V : lang_monoid} {VL : lang_monoid_laws V} .
-  Context {C : lang_module V} {CL : lang_module_laws C} .
+Definition split_sub_eval {Γ Δ} (c : conf (Δ +▶ Γ)) (e : Γ ⇒ᵥ Δ) : delay (nf∙ Δ) :=
+  eval ([ v_var , e ] ⊛ₜ c) .
 
-  Context {VA : var_assumptions} .
+Definition eval_split_sub {Γ Δ} (c : conf (Δ +▶ Γ)) (e : Γ ⇒ᵥ Δ) : delay (nf' Δ) :=
+  eval c >>= fun 'T1_0 u =>
+      match cat_split (nf_var' u) with
+      | CLeftV h => Ret' (nf_ty' u ,' (h , (nf_msg' u ,' [ v_var,  e ] ⊛ nf_val' u)))
+      | CRightV h => eval (app (e _ h) (nf_msg' u) ([v_var , e ] ⊛ nf_val' u))
+      end .
 
- Context {M : machine}.
+Lemma eval_to_msg_eq {Γ} (a b : delay (nf' Γ)) (H : a ≋ b) :
+  fmap_delay (@msg_of_nf' Γ) a ≊ fmap_delay (@msg_of_nf' Γ) b .
+Proof.
+  revert a b H; unfold it_eq; coinduction R CIH; intros a b H.
+  unfold comp_eq in H; apply it_eq_step in H.
+  cbn in *; unfold observe in H.
+  destruct (_observe a), (_observe b); dependent elimination H; econstructor.
+  - destruct r_rel as [ p [ q [ r _ ] ] ].
+    destruct r1 as [ x1 [ i1 [ m1 a1 ] ] ], r2 as [ x2 [ i2 [ m2 a2 ] ] ].
+    unfold msg_of_nf', nf_ty', nf_var', nf_msg' in *; cbn in *.
+    revert i1 m1 a1 q r; rewrite p; intros i1 m1 a1 q r.
+    now do 2 f_equal.
+  - now apply CIH.
+  - inversion q1.
+Qed.
 
-  Definition app' {Γ Δ} (u : Γ ⇒ᵥ Δ) (v : nf' Γ) : conf Δ :=
-    app (u _ (nf_var' v)) (nf_msg' v) (u ⊛ nf_val' v) .
+Lemma eval_split {Γ Δ} (c : conf (Δ +▶ Γ)) (e : Γ ⇒ᵥ Δ) :
+  split_sub_eval c e ≋ eval_split_sub c e .
+Proof.
+  unfold split_sub_eval, eval_split_sub.
+  rewrite (eval_sub c ([ v_var , e ])).
+  unfold bind_delay'.
+  remember (eval c) as t; clear c Heqt.
+  revert t; unfold comp_eq,it_eq; coinduction R CIH; cbn; intro t.
+  destruct (_observe t); [ | econstructor; apply CIH | inversion q ].
+  destruct r as [ x [ i [ m γ ] ] ]; cbn in *.
+  destruct (cat_split i).
+  + change (?u x (r_cover_l cover_cat x i)) with ((u ⊛ᵣ r_concat_l) x i).
+    rewrite s_eq_cat_l.
+    eassert (H : _) by exact (eval_nf_ret (x ,' (i , (m ,' ([v_var, e]) ⊛ γ)))).
+    unfold comp_eq in H.
+    apply it_eq_step in H; cbn in *; unfold observe in H.
+    destruct (_observe (eval (app (v_var x i) m (([v_var, e]) ⊛ γ)))); dependent elimination H; auto.
+  + change (?u x (r_cover_r cover_cat x j)) with ((u ⊛ᵣ r_concat_r) x j).
+    rewrite s_eq_cat_r.
+    destruct (_observe (eval (app (e x j) m (([v_var, e]) ⊛ γ)))); econstructor; auto.
+    now apply nf_eq_rfl'.
+Qed.
 
-  Context {ML : machine_laws} .
-
-  Lemma is_var_irr {Γ x} {v : val Γ x} (p q : is_var v) : p = q .
-    destruct p as [i1 e1], q as [i2 e2].
-    destruct (v_var_inj _ _ (eq_trans (eq_sym e1) e2)).
-    f_equal; apply YesUIP.
-  Qed.
-
-  Definition ren_is_var {Γ1 Γ2 x} (v : val Γ1 x) (e : Γ1 ⊆ Γ2) : is_var v -> is_var (e ᵣ⊛ᵥ v) .
-    intro p.
-    refine (e _ (is_var_get p) ,' _).
-    pose (i := is_var_get p); eassert (H : _) by exact (is_var_get_eq p); fold i in H |- *.
-    rewrite H; change (e ᵣ⊛ᵥ v_var x i) with ((e ᵣ⊛ v_var) x i).
-    unfold e_ren; rewrite v_sub_var; reflexivity.
-  Defined.
-
-  Variant is_var_ren_view {Γ1 Γ2 x} (v : val Γ1 x) (e : Γ1 ⊆ Γ2) : is_var (e ᵣ⊛ᵥ v) -> Type :=
-  | IsVarRen (p : is_var v) : is_var_ren_view v e (ren_is_var v e p)
-  .
-  Arguments IsVarRen {Γ1 Γ2 x v e}.
-
-  Lemma view_is_var_ren {Γ1 Γ2 x} (v : val Γ1 x) (e : Γ1 ⊆ Γ2) (p : is_var (e ᵣ⊛ᵥ v)) : is_var_ren_view v e p .
-    rewrite (is_var_irr p (ren_is_var v e (is_var_ren v e p))); econstructor.
-  Qed.
-
-(*|
-A couple derived properties on the constructed operations.
-|*)
-
-  #[global]
-  Instance e_comp_proper {Γ1 Γ2 Γ3} : Proper (ass_eq Γ2 Γ3 ==> ass_eq Γ1 Γ2 ==> ass_eq Γ1 Γ3) e_comp.
-    intros ? ? H1 ? ? H2 ? i; unfold e_comp, s_map.
-    now rewrite H1, H2.
-  Qed.
-
-  #[global]
-  Instance e_ren_proper {Γ1 Γ2 Γ3} : Proper (ass_eq Γ2 Γ3 ==> ass_eq Γ1 Γ2 ==> ass_eq Γ1 Γ3) e_ren.
-    intros ? ? H1 ? ? H2; unfold e_ren.
-    apply e_comp_proper; eauto; now rewrite H1.
-  Qed.
-
-  Lemma e_comp_ren_r {Γ1 Γ2 Γ3 Γ4} (u : Γ3 ⇒ᵥ Γ4) (v : Γ2 ⇒ᵥ Γ3) (w : Γ1 ⊆ Γ2)
-        : u ⊛ (v ⊛ᵣ w) ≡ₐ (u ⊛ v) ⊛ᵣ w .
-    reflexivity.
-  Qed.
-
-  Lemma e_comp_ren_l {Γ1 Γ2 Γ3 Γ4} (u : Γ3 ⇒ᵥ Γ4) (v : Γ2 ⊆ Γ3) (w : Γ1 ⇒ᵥ Γ2)
-        : (u ⊛ᵣ v) ⊛ w ≡ₐ u ⊛ (v ᵣ⊛ w) .
-    unfold e_ren; now rewrite v_sub_sub, e_comp_ren_r, v_sub_var.
-  Qed.
-
-  Lemma v_sub_comp {Γ1 Γ2 Γ3} (u : Γ2 ⇒ᵥ Γ3) (v : Γ1 ⇒ᵥ Γ2) {x} (w : val Γ1 x) : u ⊛ᵥ (v ⊛ᵥ w) = (u ⊛ v) ⊛ᵥ w .
-    pose (w' := s_append s_empty w : (∅ ▶ x) ⇒ᵥ Γ1).
-    change w with (w' _ Ctx.top).
-    do 2 change (?u ⊛ᵥ ?v _ Ctx.top) with ((u ⊛ v) _ Ctx.top).
-    apply v_sub_sub.
-  Qed.
-
-  Lemma v_sub_id {Γ1 Γ2} (u : Γ1 ⇒ᵥ Γ2) {x} (i : Γ1 ∋ x) : u ⊛ᵥ (v_var x i) = u x i .
-    apply v_sub_var.
-  Qed.
-
-(*|
-Evaluate a configuration inside an environment (assignment), returning only the message part (the "positive" or "static" part).
-|*)
-  Definition eval_in_env {Γ Δ} (e : Γ ⇒ᵥ Δ) (t : conf Γ) : delay (msg' Δ) :=
-    eval_to_msg (e ⊛ₜ t) .
-
-  #[global] Instance eval_in_env_proper {Γ Δ} : Proper (ass_eq Γ Δ ==> eq ==> eq) (@eval_in_env Γ Δ).
-    intros ? ? H1 ? ? H2; unfold eval_in_env; now rewrite H1, H2.
-  Qed.
-
-  Definition ciu {Γ} Δ (x y : conf Γ) : Prop
-    := forall e : Γ ⇒ᵥ Δ, eval_in_env e x ≈ eval_in_env e y.
-  Notation "x ≈⟦ciu Δ ⟧≈ y" := (ciu Δ x y) (at level 50).
-
-(*|
-Section 3: game definition
-↓+ ~ join_even
-|*)
-  Definition alt_ext : Type := ctx (context).
-  Notation "↓⁺ a" := (join_even a) (at level 9).
-  Notation "↓⁻ a" := (join_odd a) (at level 9).
-  Notation "↓[ b ] a" := (join_even_odd_aux b a) (at level 9).
-
-  Definition ogs_hg : half_game alt_ext alt_ext :=
-    {| g_move := fun es => msg' ↓⁺es ;
-       g_next := fun es m => (es ▶ dom' m) |} .
-
-  Definition ogs_g : game alt_ext alt_ext :=
-    {| g_client := ogs_hg ;
-       g_server := ogs_hg  |} .
-
-  Definition ogs_e : event alt_ext alt_ext := e_of_g ogs_g.
-
-  Definition ogs_act (Δ : context) : psh alt_ext := itree ogs_e (fun _ => msg' Δ).
-  Definition ogs_pas (Δ : context) : psh alt_ext := h_pasv ogs_hg (ogs_act Δ).
-
-  Notation "Ⓟ" := true.
-  Notation "Ⓞ" := false.
-
-(*|
-Env* (def 3.12)
-Env M Δ player es : environment part of the player (aka active at es) configuration at (Δ + es)
-Env M Δ opponent es : environment part of the opponent (aka passive at es) configuration at (Δ + es)
-|*)
-  Inductive alt_env (Δ1 Δ2 : context) : bool -> alt_ext -> Type :=
-  | ENil {b} : alt_env Δ1 Δ2 b ∅
-  | EConT {Φ Γ} : alt_env Δ2 Δ1 Ⓞ Φ -> alt_env Δ1 Δ2 Ⓟ (Φ ▶ Γ)
-  | EConF {Φ Γ} : alt_env Δ2 Δ1 Ⓟ Φ -> Γ ⇒ᵥ (Δ1 +▶ ↓⁺Φ) -> alt_env Δ1 Δ2 Ⓞ (Φ ▶ Γ)
-  .
-  Arguments ENil {Δ1 Δ2 b}.
-  Arguments EConT {Δ1 Δ2 Φ Γ}.
-  Arguments EConF {Δ1 Δ2 Φ Γ}.
-
-  Notation εₑ := (ENil) .
-  Notation "u ▶ₑ⁺" := (EConT u) (at level 40).
-  Notation "u ▶ₑ⁻ e" := (EConF u e) (at level 40).
-
-  (* flattens an alternating environment into an unstructured one *)
-  Equations concat0 {Δ1 Δ2 b Φ} (u : alt_env Δ1 Δ2 b Φ) : ↓[negb b]Φ ⇒ᵥ ((if b then Δ2 else Δ1) +▶ ↓[b]Φ) :=
-    concat0 (εₑ)     := s_empty ;
-    concat0 (u ▶ₑ⁺)   := r_concat3_1 ᵣ⊛ concat0 u ;
-    concat0 (u ▶ₑ⁻ e) := [ concat0 u , e ] .
-
-(*|
-Flattens a pair of alternating environments for both player and opponent into a "closed" substitution.
-|*)
-  Equations concat1 {Δ} Φ {b} : alt_env Δ Δ b Φ -> alt_env Δ Δ (negb b) Φ -> ↓[b]Φ ⇒ᵥ Δ :=
-    concat1 ∅       _       _         := s_empty ;
-    concat1 (Φ ▶ _) (u ▶ₑ⁺)  (v ▶ₑ⁻ e) := [ concat1 Φ u v , [ v_var , concat1 Φ v u ] ⊛ e ] ;
-    concat1 (Φ ▶ _) (u ▶ₑ⁻ e) (v ▶ₑ⁺)  := concat1 Φ u v .
-  Arguments concat1 {Δ Φ b}.
-
-(*|
-lem 4.6
-|*)
-  Lemma concat_fixpoint {Δ Φ} (u : alt_env Δ Δ Ⓟ Φ) (v : alt_env Δ Δ Ⓞ Φ)
-    :  [ v_var , concat1 u v ] ⊛ concat0 u ≡ₐ concat1 v u
-     /\ [ v_var , concat1 v u ] ⊛ concat0 v ≡ₐ concat1 u v .
-    induction Φ; dependent destruction u; dependent destruction v; cbn; split.
-    - intros ? i; dependent elimination i.
-    - intros ? i; dependent elimination i.
-    - rewrite <- e_comp_ren_l.
-      rewrite <- (proj2 (IHΦ v u)).
-      apply e_comp_proper; [ | reflexivity ].
-      symmetry; apply s_eq_cover_uniq.
-      * unfold r_concat3_1.
-        now rewrite <- s_ren_comp, 2 s_eq_cat_l.
-      * unfold r_concat3_1.
-        now rewrite <- s_ren_comp, s_eq_cat_r, s_ren_comp, s_eq_cat_r, s_eq_cat_l.
-    - symmetry; apply s_eq_cover_uniq.
-      * rewrite <- e_comp_ren_r, s_eq_cat_l.
-        symmetry; apply IHΦ.
-      * now rewrite <- e_comp_ren_r, s_eq_cat_r.
-  Qed.
-
-  Definition m_strat_act Δ : psh alt_ext := fun Φ => (conf (Δ +▶ ↓⁺Φ) * alt_env Δ Δ Ⓟ Φ)%type.
-  Definition m_strat_pas Δ : psh alt_ext := fun Φ => alt_env Δ Δ Ⓞ Φ.
-
-  Definition m_strat_wrap {Δ Φ} (x : alt_env Δ Δ Ⓟ Φ)
-     : nf' (Δ +▶ ↓⁺ Φ) -> (msg' Δ + h_actv ogs_hg (m_strat_pas Δ) Φ) :=
-      fun u =>
-        match cat_split (fst (projT2 u)) with
-        | CLeftV h => inl (_ ,' (h , nf_msg' u))
-        | CRightV h => inr ((_ ,' (h , nf_msg' u)) ,' (x ▶ₑ⁻ nf_val' u))
-        end .
-
-  Definition m_strat_play {Δ Φ} (x : m_strat_act Δ Φ)
-    : delay (msg' Δ + h_actv ogs_hg (m_strat_pas Δ) Φ)
-    := (fun _ => m_strat_wrap (snd x)) <$> eval (fst x).
-
-  Definition m_strat_resp {Δ Φ} (x : m_strat_pas Δ Φ)
-    : h_pasv ogs_hg (m_strat_act Δ) Φ
-    := fun m => (app (r_concat3_1 ᵣ⊛ᵥ concat0 x _ (fst (projT2 m)))
-                   (snd (projT2 m))
-                   (v_var ⊛ᵣ r_concat_r ⊛ᵣ r_concat_r) ,
-               x ▶ₑ⁺) .
-
-  Definition m_strat {Δ} : m_strat_act Δ ⇒ᵢ ogs_act Δ :=
-    cofix _m_strat Φ e :=
-      emb_delay (m_strat_play e) >>=
-        fun j (r : (_ @ Φ) j) =>
-          go (match r in (fiber _ b) return (itree' ogs_e (fun _ : alt_ext => msg' Δ) b) with
-              | Fib (inl m) => RetF (m : (fun _ : alt_ext => msg' Δ) Φ)
-              | Fib (inr (x ,' p)) => VisF (x : ogs_e.(e_qry) Φ)
-                                          (fun r => _m_strat (g_next r) (m_strat_resp p r))
-              end).
-
-  Lemma unfold_mstrat {Δ a} (x : m_strat_act Δ a) :
-    m_strat a x
-    ≊ (emb_delay (m_strat_play x) >>=
-        fun j (r : (_ @ a) j) =>
-          match r in (fiber _ b) return (itree ogs_e (fun _ : alt_ext => msg' Δ) b)
-          with
-          | Fib (inl m) => Ret' (m : (fun _ : alt_ext => msg' Δ) a)
-          | Fib (inr (x ,' p)) => Vis' (x : ogs_e.(e_qry) _)
-                                       (fun r => m_strat (g_next r) (m_strat_resp p r))
-          end).
-    revert a x; unfold it_eq; coinduction R CIH; intros a x.
-    cbn -[m_strat_play].
-    destruct (_observe (m_strat_play x)) as [ [ | [] ] | | [] ]; econstructor; auto.
-    eapply (ft_t (it_eq_up2bind_t _ _)); econstructor; [ reflexivity | ].
-    intros ? ? x2 ->; destruct x2 as [ [ | [] ] ]; auto.
-  Qed.
-
-  Definition m_stratp {Δ} : m_strat_pas Δ ⇒ᵢ ogs_pas Δ :=
-    fun _ x m => m_strat _ (m_strat_resp x m).
-
-  Definition m_strat_act_eqv {Δ} : relᵢ (m_strat_act Δ) (m_strat_act Δ) :=
-    fun i x y => m_strat i x ≈ m_strat i y.
-  Notation "x ≈ₐ y" := (m_strat_act_eqv _ x y) (at level 50).
-
-  Definition m_strat_pas_eqv {Δ} : relᵢ (m_strat_pas Δ) (m_strat_pas Δ) :=
-    fun i x y => forall m, m_strat_resp x m ≈ₐ m_strat_resp y m .
-  Notation "x ≈ₚ y" := (m_strat_pas_eqv _ x y) (at level 50).
-
-  Definition inj_init_act Δ {Γ} (c : conf Γ) : m_strat_act Δ (∅ ▶ Γ)
-    := ((r_concat_r ⊛ᵣ r_concat_r) ᵣ⊛ₜ c , εₑ ▶ₑ⁺).
-
-  Definition inj_init_pas {Δ Γ} (γ : Γ ⇒ᵥ Δ) : m_strat_pas Δ (∅ ▶ Γ)
-    := εₑ ▶ₑ⁻ (r_concat_l ᵣ⊛ γ).
-
-  Definition m_conf_eqv Δ : relᵢ conf conf :=
-    fun Γ u v => inj_init_act Δ u ≈ₐ inj_init_act Δ v .
-  Notation "x ≈⟦ogs Δ ⟧≈ y" := (m_conf_eqv Δ _ x y) (at level 50).
-
-  Definition reduce_t (Δ : context) : Type :=
-    ⦉ m_strat_act Δ ×ᵢ m_strat_pas Δ ⦊ᵢ .
-
-  Equations compo_body {Δ}
-    : reduce_t Δ -> delay (reduce_t Δ + msg' Δ) :=
-    compo_body x :=
-      m_strat_play (fst (projT2 x)) >>= fun _ r =>
-          match r with
-              | inl r => Ret' (inr r)
-              | inr e => Ret' (inl (_ ,' (m_strat_resp (snd (projT2 x)) (projT1 e) , (projT2 e))))
-              end.
-
-  Definition split_sub_eval {Γ Δ} (c : conf (Δ +▶ Γ)) (e : Γ ⇒ᵥ Δ) : delay (nf' Δ) :=
-    eval ([ v_var , e ] ⊛ₜ c) .
-
-  Definition eval_split_sub {Γ Δ} (c : conf (Δ +▶ Γ)) (e : Γ ⇒ᵥ Δ) : delay (nf' Δ) :=
-    eval c >>= fun 'T1_0 u =>
-        match cat_split (nf_var' u) with
-        | CLeftV h => Ret' (nf_ty' u ,' (h , (nf_msg' u ,' [ v_var,  e ] ⊛ nf_val' u)))
-        | CRightV h => eval (app (e _ h) (nf_msg' u) ([v_var , e ] ⊛ nf_val' u))
-        end .
-
-  #[global] Instance nf_eq_rfl {Γ t} : Reflexive (@nf_eq Γ t) .
-    intros a; exists eq_refl; auto.
-  Qed.
-
-  #[global] Instance nf_eq_sym {Γ t} : Symmetric (@nf_eq Γ t) .
-    intros a b [ p q ].
-    unshelve econstructor.
-    - now symmetry.
-    - intros ? i.
-      destruct a as [ m a ] ; cbn in *.
-      revert a q i; rewrite p; clear p; intros a q i.
-      symmetry; apply q.
-  Qed.
-
-  #[global] Instance nf_eq_tra {Γ t} : Transitive (@nf_eq Γ t) .
-    intros a b c [ p1 q1 ] [ p2 q2 ].
-    unfold nf_eq.
-    unshelve econstructor.
-    - now transitivity (projT1 b).
-    - transitivity (rew [fun m : msg t => dom m ⇒ᵥ Γ] p2 in projT2 b); auto.
-      now rewrite <- p2.
-  Qed.
-
-  #[global] Instance nf_eq_rfl' {Γ} : Reflexiveᵢ (fun _ : T1 => @nf_eq' Γ) .
-    intros _ [ x [ i n ] ].
-    unshelve econstructor; auto.
-  Qed.
-
-  #[global] Instance nf_eq_sym' {Γ} : Symmetricᵢ (fun _ : T1 => @nf_eq' Γ) .
-    intros _ [ x1 [ i1 n1 ] ] [ x2 [ i2 n2 ] ] [ p [ q1 q2 ] ].
-    unshelve econstructor; [ | split ]; cbn in *.
-    - now symmetry.
-    - revert i1 q1; rewrite p; intros i1 q1; now symmetry.
-    - revert n1 q2; rewrite p; intros n1 q2; now symmetry.
-  Qed.
-
-  #[global] Instance nf_eq_tra' {Γ} : Transitiveᵢ (fun _ : T1 => @nf_eq' Γ) .
-    intros _ [ x1 [ i1 n1 ] ] [ x2 [ i2 n2 ] ] [ x3 [ i3 n3 ] ] [ p1 [ q1 r1 ] ] [ p2 [ q2 r2 ] ].
-    unshelve econstructor; [ | split ]; cbn in *.
-    - now transitivity x2.
-    - transitivity (rew [has Γ] p2 in i2); auto.
-      now rewrite <- p2.
-    - transitivity (rew [nf Γ] p2 in n2); auto.
-      now rewrite <- p2.
-  Qed.
-
-  Lemma eval_to_msg_eq {Γ} (a b : delay (nf' Γ)) (H : a ≋ b) :
-    fmap_delay (@msg_of_nf' Γ) a ≊ fmap_delay (@msg_of_nf' Γ) b .
-    revert a b H; unfold it_eq; coinduction R CIH; intros a b H.
-    unfold comp_eq in H; apply it_eq_step in H.
-    cbn in *; unfold observe in H.
-    destruct (_observe a), (_observe b); dependent elimination H; econstructor.
-    - destruct r_rel as [ p [ q [ r _ ] ] ].
-      destruct r1 as [ x1 [ i1 [ m1 a1 ] ] ], r2 as [ x2 [ i2 [ m2 a2 ] ] ].
-      unfold msg_of_nf', nf_ty', nf_var', nf_msg' in *; cbn in *.
-      revert i1 m1 a1 q r; rewrite p; intros i1 m1 a1 q r.
-      now do 2 f_equal.
-    - now apply CIH.
-    - inversion q1.
-  Qed.
-
-  Lemma eval_split {Γ Δ} (c : conf (Δ +▶ Γ)) (e : Γ ⇒ᵥ Δ) : split_sub_eval c e ≋ eval_split_sub c e .
-    unfold split_sub_eval, eval_split_sub.
-    rewrite (eval_sub c ([ v_var , e ])).
-    unfold bind_delay'.
-    remember (eval c) as t; clear c Heqt.
-    revert t; unfold comp_eq,it_eq; coinduction R CIH; cbn; intro t.
-    destruct (_observe t); [ | econstructor; apply CIH | inversion q ].
-    destruct r as [ x [ i [ m γ ] ] ]; cbn in *.
-    destruct (cat_split i).
-    + change (?u x (r_cover_l cover_cat x i)) with ((u ⊛ᵣ r_concat_l) x i).
-      rewrite s_eq_cat_l.
-      eassert (H : _) by exact (eval_nf_ret (x ,' (i , (m ,' ([v_var, e]) ⊛ γ)))).
-      unfold comp_eq in H.
-      apply it_eq_step in H; cbn in *; unfold observe in H.
-      destruct (_observe (eval (app (v_var x i) m (([v_var, e]) ⊛ γ)))); dependent elimination H; auto.
-    + change (?u x (r_cover_r cover_cat x j)) with ((u ⊛ᵣ r_concat_r) x j).
-      rewrite s_eq_cat_r.
-      destruct (_observe (eval (app (e x j) m (([v_var, e]) ⊛ γ)))); econstructor; auto.
-      now apply nf_eq_rfl'.
-  Qed.
-
-  Definition compo {Δ a} (u : m_strat_act Δ a) (v : m_strat_pas Δ a) : delay (msg' Δ)
-    := iter_delay compo_body (a ,' (u , v)).
-  Notation "u ∥ v" := (compo u v) (at level 40).
-
-  (* guilhem: rename? *)
-  Definition barb {Γ} Δ (x y : conf Γ) : Prop
-    := forall e : Γ ⇒ᵥ Δ, (inj_init_act Δ x ∥ inj_init_pas e) ≈ (inj_init_act Δ y ∥ inj_init_pas e).
-  Notation "x ≈⟦barb Δ ⟧≈ y" := (barb Δ x y) (at level 50).
-
-  Equations reduce {Δ} : reduce_t Δ -> delay (msg' Δ) :=
-    reduce u := eval_in_env
-                       ([ v_var , concat1 (snd (fst (projT2 u))) (snd (projT2 u)) ])
-                       (fst (fst (projT2 u))) .
+Equations reduce {Δ} : reduce_t Δ -> delay (msg' Δ) :=
+  reduce u := eval_in_env
+                ([ v_var , concat1 (snd (fst (projT2 u))) (snd (projT2 u)) ])
+                (fst (fst (projT2 u))) .
 
   Definition reduce' {Δ} : forall i, reduce_t Δ -> itree ∅ₑ (fun _ : T1 => msg' Δ) i := fun 'T1_0 => reduce .
 
@@ -602,7 +301,8 @@ lem 4.6
 
 
   Lemma quatre_trois {Δ a} (c : m_strat_act Δ a) (e : m_strat_pas Δ a)
-    : reduce (_ ,' (c , e)) ≊ (c ∥g e) .
+    : reduce (_ ,' (c , e)) ≊ (c ∥g e).
+  Proof.
     refine (iter_evg_uniq (fun 'T1_0 u => compo_body u) (fun 'T1_0 u => reduce u) _ _ T1_0 _).
     clear a c e; intros [] [ ? [ u v ] ].
     etransitivity; [ | symmetry; apply quatre_trois_pre ].
@@ -643,10 +343,11 @@ lem 4.6
         now rewrite s_eq_cat_l, s_ren_comp, s_eq_cat_r, s_eq_cat_l.
       + erewrite app_proper; [ reflexivity | ].
         now rewrite q, 2 e_comp_ren_r, v_sub_var, 2 s_eq_cat_r.
-   Qed.
+  Qed.
 
-  Lemma quatre_trois_app {Γ Δ} (c : conf Γ) (e : Γ ⇒ᵥ Δ)
-        : eval_in_env e c ≊ (inj_init_act Δ c ∥g inj_init_pas e).
+  Lemma quatre_trois_app {Γ Δ} (c : conf Γ) (e : Γ ⇒ᵥ Δ) :
+    eval_in_env e c ≊ (inj_init_act Δ c ∥g inj_init_pas e).
+  Proof.
     etransitivity; [ | apply quatre_trois ].
     unfold reduce, inj_init_act, eval_in_env; cbn [fst snd projT1 projT2]; apply (fmap_eq (RX:=eqᵢ _)).
     intros ? ? ? ->; auto.
@@ -658,6 +359,26 @@ lem 4.6
     unfold e_ren, r_concat_l, cover_cat; cbn; rewrite r_cover_l_nil, s_ren_id.
     now rewrite 2 v_var_sub.
   Qed.
+
+(*|
+Evaluate a configuration inside an environment (assignment), returning only the message part (the "positive" or "static" part).
+|*)
+  Definition eval_in_env {Γ Δ} (e : Γ ⇒ᵥ Δ) (t : conf Γ) : delay (msg' Δ) :=
+    eval_to_msg (e ⊛ₜ t) .
+
+  #[global] Instance eval_in_env_proper {Γ Δ} : Proper (ass_eq Γ Δ ==> eq ==> eq) (@eval_in_env Γ Δ).
+    intros ? ? H1 ? ? H2; unfold eval_in_env; now rewrite H1, H2.
+  Qed.
+
+  Definition ciu {Γ} Δ (x y : conf Γ) : Prop
+    := forall e : Γ ⇒ᵥ Δ, eval_in_env e x ≈ eval_in_env e y.
+  Notation "x ≈⟦ciu Δ ⟧≈ y" := (ciu Δ x y) (at level 50).
+
+  (* guilhem: rename? *)
+  Definition barb {Γ} Δ (x y : conf Γ) : Prop
+    := forall e : Γ ⇒ᵥ Δ, (inj_init_act Δ x ∥ inj_init_pas e) ≈ (inj_init_act Δ y ∥ inj_init_pas e).
+  Notation "x ≈⟦barb Δ ⟧≈ y" := (barb Δ x y) (at level 50).
+
 
   Theorem barb_correction {Γ} Δ (x y : conf Γ) : x ≈⟦barb Δ ⟧≈ y -> x ≈⟦ciu Δ ⟧≈ y.
     intros H e.
@@ -773,6 +494,7 @@ lem 4.6
   Qed.
 
   Theorem ogs_correction {Γ} Δ (x y : conf Γ) : x ≈⟦ogs Δ ⟧≈ y -> x ≈⟦ciu Δ ⟧≈ y.
+  Proof.
     intro H; apply barb_correction.
     intro e; unfold compo.
     change (iter _ T1_0 ?u) with (iter_delay compo_body u); rewrite <- 2 compo_compo_alt.
