theories/OGS/Game.v
@@ -1,0 +1,56 @@
+From OGS Require Import Prelude.
+From OGS.Utils Require Import Ctx Rel.
+From OGS.Game Require Import HalfGame Event.
+From OGS.OGS Require Import Subst Obs Machine.
+From OGS.ITree Require Import ITree Eq Delay Structure Properties Guarded.
+
+Section withFam.
+
+(*|
+We consider a language abstractly captured as a machine
+|*)
+  Context {bT : baseT}.
+  Context {bV : baseV}.
+  Context {bC : baseC}.
+  Context {sV : subst_monoid bV}.
+  Context {sC : subst_module bV bC}.
+  Context {oS : observation_structure}.
+  Context {M: machine}.
+(*|
+Satisfying an appropriate axiomatization
+|*)
+  Context {sVL: subst_monoid_laws}.
+  Context {sCL: subst_module_laws}.
+  Context {VA : var_assumptions} .
+  Context {ML: machine_laws}.
+
+(*|
+Section 3: game definition
+↓+ ~ join_even
+|*)
+  Definition alt_ext : Type := ctx (context).
+  Notation "↓⁺ a" := (join_even a) (at level 9).
+  Notation "↓⁻ a" := (join_odd a) (at level 9).
+  Notation "↓[ b ] a" := (join_even_odd_aux b a) (at level 9).
+
+  Definition ogs_hg : half_game alt_ext alt_ext :=
+    {| g_move := fun es => obs∙ ↓⁺es ;
+       g_next := fun es m => (es ▶ dom∙ m) |} .
+
+  Definition ogs_g : game alt_ext alt_ext :=
+    {| g_client := ogs_hg ;
+       g_server := ogs_hg  |} .
+
+  Definition ogs_e : event alt_ext alt_ext := e_of_g ogs_g.
+
+  Definition ogs_act (Δ : context) : psh alt_ext := itree ogs_e (fun _ => obs∙ Δ).
+  Definition ogs_pas (Δ : context) : psh alt_ext := h_pasv ogs_hg (ogs_act Δ).
+
+End withFam.
+
+Notation "↓⁺ a" := (join_even a) (at level 9).
+Notation "↓⁻ a" := (join_odd a) (at level 9).
+Notation "↓[ b ] a" := (join_even_odd_aux b a) (at level 9).
+Notation "Ⓟ" := true.
+Notation "Ⓞ" := false.
+
