theories/OGS/Soundness.v
@@ -1,0 +1,182 @@
+From OGS Require Import Prelude.
+From OGS.Utils Require Import Ctx Rel.
+From OGS.Game Require Import HalfGame Event.
+From OGS.OGS Require Import Subst Obs Machine Game Strategy.
+From OGS.ITree Require Import ITree Eq Delay Structure Properties Guarded.
+
+Open Scope ctx_scope.
+
+Section withFam.
+
+(*|
+We consider a language abstractly captured as a machine
+|*)
+  Context {bT : baseT}.
+  Context {bV : baseV}.
+  Context {bC : baseC}.
+  Context {sV : subst_monoid bV}.
+  Context {sC : subst_module bV bC}.
+  Context {oS : observation_structure}.
+  Context {M: machine}.
+(*|
+Satisfying an appropriate axiomatization
+|*)
+  Context {sVL: subst_monoid_laws}.
+  Context {sCL: subst_module_laws}.
+  Context {VA : var_assumptions} .
+  Context {ML: machine_laws}.
+
+(*|
+Evaluate a configuration inside an environment (assignment), returning only the message part (the "positive" or "static" part).
+|*)
+  Definition eval_in_env {Γ Δ} (e : Γ ⇒ᵥ Δ) (t : conf Γ) : delay (obs∙ Δ) :=
+    eval_to_obs (e ⊛ₜ t) .
+
+  #[global] Instance eval_in_env_proper {Γ Δ} : Proper (ass_eq Γ Δ ==> eq ==> eq) (@eval_in_env Γ Δ).
+    intros ? ? H1 ? ? H2; unfold eval_in_env; now rewrite H1, H2.
+  Qed.
+
+  Definition ciu {Γ} Δ (x y : conf Γ) : Prop
+    := forall e : Γ ⇒ᵥ Δ, eval_in_env e x ≈ eval_in_env e y.
+  Notation "x ≈⟦ciu Δ ⟧≈ y" := (ciu Δ x y) (at level 50).
+
+  Lemma compo_body_guarded_aux {Δ Ψ} (u : alt_env Δ Δ Ⓟ Ψ) (v : alt_env Δ Δ Ⓞ Ψ)
+    {x} (m : obs x) (γ : dom m ⇒ᵥ (Δ +▶ ↓⁺ Ψ)) (j : ↓⁺ Ψ ∋ x) :
+    ev_guarded (fun 'T1_0 => compo_body (Δ := Δ))
+      (compo_body ((Ψ ▶ dom m),' (app (r_concat3_1 ᵣ⊛ᵥ concat0 v x j) m ((v_var ⊛ᵣ r_concat_r) ⊛ᵣ r_concat_r), v ▶ₑ⁺, u ▶ₑ⁻ γ))) .
+  Proof.
+    pose (m' := (x ,' m)).
+    revert γ j.
+    change x with (projT1 m').
+    change m with (projT2 m').
+    remember m' as m''; clear m' m x Heqm''; rename m'' into m.
+    pose (wf := eval_app_not_var m).
+
+    revert Ψ u v; induction wf; intros Ψ u v γ j.
+    destruct x as [ x m ]; cbn [projT1 projT2] in *.
+
+    pose (h := lt_wf (var_height j)); remember (var_height j) as n.
+    revert Ψ u v γ j Heqn; induction h; intros Ψ u v γ j Heqn.
+
+    unfold ev_guarded; cbn -[cat_split].
+
+    pose (vv := @r_concat3_1 typ Δ ↓⁻ Ψ (@dom S x m) ᵣ⊛ᵥ concat0 v x j).
+    change (r_concat3_1 ᵣ⊛ᵥ _) with vv; destruct (is_var_dec vv).
+
+    - destruct i as [ i eq ].
+      rewrite eq.
+      eassert (H3 : _) by exact (eval_nf_ret (_ ,' (i , (m ,' ((v_var ⊛ᵣ r_concat_r) ⊛ᵣ r_concat_r))))).
+      unfold comp_eq in H3.
+      apply it_eq_step in H3; cbn in H3; unfold observe in H3.
+      pose (ot := _observe (eval (app (v_var x i) m ((v_var ⊛ᵣ r_concat_r) ⊛ᵣ r_concat_r)))); fold ot in H3 |- *.
+      destruct ot; dependent elimination H3.
+      cbn in r1, r_rel |- * .
+      destruct r1 as [ x' [ i' [ m' a' ] ] ].
+      destruct r_rel as [ p [ q r ] ]; cbn in *.
+      unfold m_strat_wrap; unfold dom' in a'; unfold msg_of_nf', nf_ty', nf_var', nf_msg' in *; cbn [ fst snd projT1 projT2] in *.
+      revert i' m' a' q r; rewrite p; clear p x'; intros i' m' a' q [ r1 _ ]; cbn in q, r1.
+      rewrite q; clear q i'.
+      revert a'; rewrite r1; clear r1 m'; intros a'.
+      pose (i' := (i ,' eq) : is_var vv).
+      change i with (is_var_get i').
+      remember i' as ii; clear i i' Heqii eq.
+      unfold vv in ii; destruct (view_is_var_ren _ _ ii).
+      destruct p; simpl is_var_get.
+      destruct (cat_split x1).
+      * unfold r_concat3_1; change (?u x (r_cover_l _ x i)) with ((u ⊛ᵣ r_concat_l) x i).
+        rewrite s_eq_cat_l, cat_split_l.
+        now do 2 econstructor.
+      * unfold r_concat3_1; change (?u x (r_cover_r _ x j0)) with ((u ⊛ᵣ r_concat_r) x j0).
+        rewrite s_eq_cat_r; unfold s_ren, s_map; rewrite cat_split_r.
+        unfold dom', m_strat_resp; cbn [fst snd projT1 projT2].
+        refine (GNext _); eapply H2; [ | reflexivity ].
+
+        rewrite Heqn.
+        unfold var_height; rewrite var_depth_ext.
+        simpl c_length; rewrite PeanoNat.Nat.sub_succ.
+        apply (Plus.plus_lt_reg_l_stt _ _ (var_depth j0 + var_depth j)).
+        rewrite PeanoNat.Nat.add_shuffle0.
+        rewrite Arith_prebase.le_plus_minus_r_stt; [ | exact (@var_depth_le _ false _ j0) ].
+        rewrite <- PeanoNat.Nat.add_assoc.
+        rewrite Arith_prebase.le_plus_minus_r_stt; [ | exact (@var_depth_le Ψ _ _ j) ].
+        rewrite PeanoNat.Nat.add_comm.
+        apply Plus.plus_lt_compat_r_stt.
+        exact (depth_increases v j j0 e).
+
+    - remember (eval (app vv m ((v_var ⊛ᵣ r_concat_r) ⊛ᵣ r_concat_r))) as t.
+      remember (_observe t) as ot.
+      destruct ot; try now do 2 econstructor.
+      unfold m_strat_wrap.
+      destruct r as [ x' [ j' [ m' a' ]]]. unfold nf_msg', nf_val' in *. cbn [ fst snd projT1 projT2 ].
+      pose (uu := cat_split j'); change (cat_split j') with uu; destruct uu.
+      now do 2 econstructor.
+      refine (GNext _).
+      unfold dom', msg_msg'; cbn [fst snd projT1 projT2].
+      eapply (H0 (x' ,' m')).
+      econstructor.
+      exact f.
+      apply it_eq_unstep; cbn.
+      rewrite Heqt in Heqot.
+      rewrite <- Heqot.
+      econstructor; reflexivity.
+  Qed.
+
+
+  Lemma compo_body_guarded {Δ} : eqn_ev_guarded (fun 'T1_0 => compo_body (Δ := Δ)).
+    intros [] [ Γ [ [c u] v ] ]; unfold m_strat_pas in v.
+    unfold ev_guarded; cbn -[cat_split].
+    pose (ot := _observe (eval c)); change (_observe (eval c)) with ot.
+    destruct ot; try now do 2 econstructor.
+    remember r as r'; rewrite Heqr'.
+    unfold m_strat_wrap; destruct r as [ ? [ i [ m γ ] ] ]; cbn in *.
+    destruct (cat_split i); try now do 2 econstructor.
+    refine (GNext _).
+    unfold obs'_dom, obs'_obs, obs'_ty; cbn [ fst snd projT1 projT2 ].
+    apply compo_body_guarded_aux.
+  Qed.
+
+  Definition compo_ev_guarded {Δ a} (u : m_strat_act Δ a) (v : m_strat_pas Δ a) : delay (msg' Δ)
+    := iter_ev_guarded _ compo_body_guarded T1_0 (a ,' (u , v)).
+  Notation "u ∥g v" := (compo_ev_guarded u v) (at level 40).
+
+  Lemma quatre_trois_app {Γ Δ} (c : conf Γ) (e : Γ ⇒ᵥ Δ) :
+    eval_in_env e c ≊ (inj_init_act Δ c ∥g inj_init_pas e).
+  Proof.
+    etransitivity; [ | apply quatre_trois ].
+    unfold reduce, inj_init_act, eval_in_env; cbn [fst snd projT1 projT2]; apply (fmap_eq (RX:=eqᵢ _)).
+    intros ? ? ? ->; auto.
+    unfold inj_init_pas; rewrite concat1_equation_2, 2 concat1_equation_1.
+    unfold c_ren; rewrite c_sub_sub, c_sub_proper ; try reflexivity.
+    rewrite s_eq_cover_empty_r.
+    rewrite e_comp_ren_r, v_sub_var.
+    rewrite s_ren_comp, 2 s_eq_cat_r.
+    unfold e_ren, r_concat_l, cover_cat; cbn; rewrite r_cover_l_nil, s_ren_id.
+    now rewrite 2 v_var_sub.
+  Qed.
+
+  Definition barb {Γ} Δ (x y : conf Γ) : Prop
+    := forall e : Γ ⇒ᵥ Δ, (inj_init_act Δ x ∥ inj_init_pas e) ≈ (inj_init_act Δ y ∥ inj_init_pas e).
+  Notation "x ≈⟦barb Δ ⟧≈ y" := (barb Δ x y) (at level 50).
+
+  Theorem barb_correction {Γ} Δ (x y : conf Γ) : x ≈⟦barb Δ ⟧≈ y -> x ≈⟦ciu Δ ⟧≈ y.
+  Proof.
+    intros H e.
+    etransitivity; [ apply it_eq_wbisim, (quatre_trois_app x e) | ].
+    etransitivity; [ apply iter_evg_iter | ].
+    etransitivity; [ apply (H e) | symmetry ].
+    etransitivity; [ apply it_eq_wbisim, (quatre_trois_app y e) | ].
+    etransitivity; [ apply iter_evg_iter | ].
+    reflexivity.
+  Qed.
+
+  Theorem ogs_correction {Γ} Δ (x y : conf Γ) : x ≈⟦ogs Δ ⟧≈ y -> x ≈⟦ciu Δ ⟧≈ y.
+  Proof.
+    intro H; apply barb_correction.
+    intro e; unfold compo.
+    change (iter _ T1_0 ?u) with (iter_delay compo_body u); rewrite <- 2 compo_compo_alt.
+    apply compo_alt_proper; [ exact H | intro; reflexivity ].
+  Qed.
+
+End withInteractionSpec.
+About ogs_correction.
+Print Assumptions ogs_correction.
