theories/OGS/Strategy.v
@@ -1,0 +1,180 @@
+From Coinduction Require Import coinduction tactics.
+
+From OGS Require Import Prelude.
+From OGS.Utils Require Import Ctx Rel.
+From OGS.Game Require Import HalfGame Event.
+From OGS.OGS Require Import Subst Obs Machine Game Utility_lemmas.
+From OGS.ITree Require Import ITree Eq Delay Structure Properties Guarded.
+
+Section withFam.
+
+(*|
+We consider a language abstractly captured as a machine
+|*)
+  Context {bT : baseT}.
+  Context {bV : baseV}.
+  Context {bC : baseC}.
+  Context {sV : subst_monoid bV}.
+  Context {sC : subst_module bV bC}.
+  Context {oS : observation_structure}.
+  Context {M: machine}.
+(*|
+Satisfying an appropriate axiomatization
+|*)
+  Context {sVL: subst_monoid_laws}.
+  Context {sCL: subst_module_laws}.
+  Context {VA : var_assumptions} .
+  Context {ML: machine_laws}.
+
+(*|
+Env*
+Env M Δ player es : environment part of the player (aka active at es) configuration at (Δ + es)
+Env M Δ opponent es : environment part of the opponent (aka passive at es) configuration at (Δ + es)
+|*)
+  Inductive alt_env (Δ1 Δ2 : context) : bool -> alt_ext -> Type :=
+  | ENil {b} : alt_env Δ1 Δ2 b ∅
+  | EConT {Φ Γ} : alt_env Δ2 Δ1 Ⓞ Φ -> alt_env Δ1 Δ2 Ⓟ (Φ ▶ Γ)
+  | EConF {Φ Γ} : alt_env Δ2 Δ1 Ⓟ Φ -> Γ ⇒ᵥ (Δ1 +▶ ↓⁺Φ) -> alt_env Δ1 Δ2 Ⓞ (Φ ▶ Γ)
+  .
+  Arguments ENil {Δ1 Δ2 b}.
+  Arguments EConT {Δ1 Δ2 Φ Γ}.
+  Arguments EConF {Δ1 Δ2 Φ Γ}.
+
+  Notation εₑ := (ENil) .
+  Notation "u ▶ₑ⁺" := (EConT u) (at level 40).
+  Notation "u ▶ₑ⁻ e" := (EConF u e) (at level 40).
+
+  (* flattens an alternating environment into an unstructured one *)
+  Equations concat0 {Δ1 Δ2 b Φ} (u : alt_env Δ1 Δ2 b Φ) : ↓[negb b]Φ ⇒ᵥ ((if b then Δ2 else Δ1) +▶ ↓[b]Φ) :=
+    concat0 (εₑ)     := a_empty ;
+    concat0 (u ▶ₑ⁺)   := r_concat3_1 ᵣ⊛ concat0 u ;
+    concat0 (u ▶ₑ⁻ e) := [ concat0 u , e ] .
+
+(*|
+Flattens a pair of alternating environments for both player and opponent into a "closed" substitution.
+|*)
+  Equations concat1 {Δ} Φ {b} : alt_env Δ Δ b Φ -> alt_env Δ Δ (negb b) Φ -> ↓[b]Φ ⇒ᵥ Δ :=
+    concat1 ∅       _       _         := a_empty ;
+    concat1 (Φ ▶ _) (u ▶ₑ⁺)  (v ▶ₑ⁻ e) := [ concat1 Φ u v , [ v_var , concat1 Φ v u ] ⊛ e ] ;
+    concat1 (Φ ▶ _) (u ▶ₑ⁻ e) (v ▶ₑ⁺)  := concat1 Φ u v .
+  Arguments concat1 {Δ Φ b}.
+
+(*|
+
+|*)
+  Lemma concat_fixpoint {Δ Φ} (u : alt_env Δ Δ Ⓟ Φ) (v : alt_env Δ Δ Ⓞ Φ)
+    :  [ v_var , concat1 u v ] ⊛ concat0 u ≡ₐ concat1 v u
+     /\ [ v_var , concat1 v u ] ⊛ concat0 v ≡ₐ concat1 u v .
+    induction Φ; dependent destruction u; dependent destruction v; cbn; split.
+    - cbn. intros ? i; dependent elimination i.
+    - intros ? i; dependent elimination i.
+    - simp concat1.
+      rewrite <- e_comp_ren_l.
+      rewrite <- (proj2 (IHΦ v u)).
+      apply e_comp_proper; [ | reflexivity ].
+      symmetry; apply s_eq_cover_uniq.
+      * unfold r_concat3_1.
+        now rewrite <- s_ren_comp, 2 s_eq_cat_l.
+      * unfold r_concat3_1.
+        now rewrite <- s_ren_comp, s_eq_cat_r, s_ren_comp, s_eq_cat_r, s_eq_cat_l.
+    - simp concat1. symmetry; apply s_eq_cover_uniq.
+      * rewrite <- e_comp_ren_r, s_eq_cat_l.
+        symmetry; apply IHΦ.
+      * now rewrite <- e_comp_ren_r, s_eq_cat_r.
+  Qed.
+
+  Definition m_strat_act Δ : psh alt_ext := fun Φ => (conf (Δ +▶ ↓⁺Φ) * alt_env Δ Δ Ⓟ Φ)%type.
+  Definition m_strat_pas Δ : psh alt_ext := fun Φ => alt_env Δ Δ Ⓞ Φ.
+
+  Definition m_strat_wrap {Δ Φ} (x : alt_env Δ Δ Ⓟ Φ)
+     : nf' (Δ +▶ ↓⁺ Φ) -> (obs∙ Δ + h_actv ogs_hg (m_strat_pas Δ) Φ) :=
+      fun u =>
+        match cat_split (fst (projT2 u)) with
+        | CLeftV h => inl (_ ,' (h , nf'_obs u))
+        | CRightV h => inr ((_ ,' (h , nf'_obs u)) ,' (x ▶ₑ⁻ nf'_val u))
+        end .
+
+  Definition m_strat_play {Δ Φ} (x : m_strat_act Δ Φ)
+    : delay (obs∙ Δ + h_actv ogs_hg (m_strat_pas Δ) Φ)
+    := (fun _ => m_strat_wrap (snd x)) <$> eval (fst x).
+
+  Definition m_strat_resp {Δ Φ} (x : m_strat_pas Δ Φ)
+    : h_pasv ogs_hg (m_strat_act Δ) Φ
+    := fun m => (app (r_concat3_1 ᵣ⊛ᵥ concat0 x _ (fst (projT2 m)))
+                   (snd (projT2 m))
+                   (v_var ⊛ᵣ r_concat_r ⊛ᵣ r_concat_r) ,
+               x ▶ₑ⁺) .
+
+  Definition m_strat {Δ} : m_strat_act Δ ⇒ᵢ ogs_act Δ :=
+    cofix _m_strat Φ e :=
+      emb_delay (m_strat_play e) >>=
+        fun j (r : (_ @ Φ) j) =>
+          go (match r in (fiber _ b) return (itree' ogs_e (fun _ : alt_ext => obs∙ Δ) b) with
+              | Fib (inl m) => RetF (m : (fun _ : alt_ext => obs∙ Δ) Φ)
+              | Fib (inr (x ,' p)) => VisF (x : ogs_e.(e_qry) Φ)
+                                          (fun r => _m_strat (g_next r) (m_strat_resp p r))
+              end).
+
+  Lemma unfold_mstrat {Δ a} (x : m_strat_act Δ a) :
+    m_strat a x
+    ≊ (emb_delay (m_strat_play x) >>=
+        fun j (r : (_ @ a) j) =>
+          match r in (fiber _ b) return (itree ogs_e (fun _ : alt_ext => obs∙ Δ) b)
+          with
+          | Fib (inl m) => Ret' (m : (fun _ : alt_ext => obs∙ Δ) a)
+          | Fib (inr (x ,' p)) => Vis' (x : ogs_e.(e_qry) _)
+                                       (fun r => m_strat (g_next r) (m_strat_resp p r))
+          end).
+    revert a x; unfold it_eq; coinduction R CIH; intros a x.
+    cbn -[m_strat_play].
+    destruct (_observe (m_strat_play x)) as [ [ | [] ] | | [] ]; econstructor; auto.
+    eapply (ft_t (it_eq_up2bind_t _ _)); econstructor; [ reflexivity | ].
+    intros ? ? x2 ->; destruct x2 as [ [ | [] ] ]; auto.
+  Qed.
+
+  Definition m_stratp {Δ} : m_strat_pas Δ ⇒ᵢ ogs_pas Δ :=
+    fun _ x m => m_strat _ (m_strat_resp x m).
+
+  Definition m_strat_act_eqv {Δ} : relᵢ (m_strat_act Δ) (m_strat_act Δ) :=
+    fun i x y => m_strat i x ≈ m_strat i y.
+  Notation "x ≈ₐ y" := (m_strat_act_eqv _ x y) (at level 50).
+
+  Definition m_strat_pas_eqv {Δ} : relᵢ (m_strat_pas Δ) (m_strat_pas Δ) :=
+    fun i x y => forall m, m_strat_resp x m ≈ₐ m_strat_resp y m .
+  Notation "x ≈ₚ y" := (m_strat_pas_eqv _ x y) (at level 50).
+
+  Definition inj_init_act Δ {Γ} (c : conf Γ) : m_strat_act Δ (∅ ▶ Γ) :=
+    ((r_concat_r ⊛ᵣ r_concat_r) ᵣ⊛ₜ c , εₑ ▶ₑ⁺).
+
+  Definition inj_init_pas {Δ Γ} (γ : Γ ⇒ᵥ Δ) : m_strat_pas Δ (∅ ▶ Γ) :=
+    εₑ ▶ₑ⁻ (r_concat_l ᵣ⊛ γ).
+
+  Definition m_conf_eqv Δ : relᵢ conf conf :=
+    fun Γ u v => inj_init_act Δ u ≈ₐ inj_init_act Δ v .
+  Notation "x ≈⟦ogs Δ ⟧≈ y" := (m_conf_eqv Δ _ x y) (at level 50).
+
+  Definition reduce_t (Δ : context) : Type :=
+    ⦉ m_strat_act Δ ×ᵢ m_strat_pas Δ ⦊ᵢ .
+
+  Equations compo_body {Δ} : reduce_t Δ -> delay (reduce_t Δ + obs∙ Δ) :=
+    compo_body x :=
+      m_strat_play (fst (projT2 x)) >>= fun _ r =>
+          match r with
+          | inl r => Ret' (inr r)
+          | inr e => Ret' (inl (_ ,' (m_strat_resp (snd (projT2 x)) (projT1 e) , (projT2 e))))
+          end.
+
+  Definition compo {Δ a} (u : m_strat_act Δ a) (v : m_strat_pas Δ a) :
+    delay (obs∙ Δ) :=
+    iter_delay compo_body (a ,' (u , v)).
+  Notation "u ∥ v" := (compo u v) (at level 40).
+
+End withFam.
+
+#[global] Notation εₑ := (ENil) .
+#[global] Notation "u ▶ₑ⁺" := (EConT u) (at level 40).
+#[global] Notation "u ▶ₑ⁻ e" := (EConF u e) (at level 40).
+#[global] Notation "x ≈ₐ y" := (m_strat_act_eqv _ x y) (at level 50).
+#[global] Notation "x ≈ₚ y" := (m_strat_pas_eqv _ x y) (at level 50).
+#[global] Notation "u ∥ v" := (compo u v) (at level 40).
+#[global] Notation "x ≈⟦ogs Δ ⟧≈ y" := (m_conf_eqv Δ _ x y) (at level 50).
