theories/OGS/Utility_lemmas.v
@@ -1,0 +1,96 @@
+From OGS Require Import Prelude.
+From OGS.Utils Require Import Ctx Rel.
+From OGS.Game Require Import HalfGame Event.
+From OGS.OGS Require Import Subst Obs Machine.
+From OGS.ITree Require Import ITree Eq Delay Structure Properties Guarded.
+
+Section withFam.
+
+(*|
+We consider a language abstractly captured as a machine
+|*)
+  Context {bT : baseT}.
+  Context {bV : baseV}.
+  Context {bC : baseC}.
+  Context {sV : subst_monoid bV}.
+  Context {sC : subst_module bV bC}.
+  Context {oS : observation_structure}.
+  Context {M: machine}.
+(*|
+Satisfying an appropriate axiomatization
+|*)
+  Context {sVL: subst_monoid_laws}.
+  Context {sCL: subst_module_laws}.
+  Context {VA : var_assumptions} .
+  Context {ML: machine_laws}.
+
+  Lemma is_var_irr {Γ x} {v : val Γ x} (p q : is_var v) : p = q.
+  Proof.
+    destruct p as [i1 e1], q as [i2 e2].
+    destruct (v_var_inj _ _ (eq_trans (eq_sym e1) e2)).
+    f_equal; apply YesUIP.
+  Qed.
+
+  Definition ren_is_var {Γ1 Γ2 x} (v : val Γ1 x) (e : Γ1 ⊆ Γ2) : is_var v -> is_var (e ᵣ⊛ᵥ v).
+  Proof.
+    intro p.
+    refine (e _ (is_var_get p) ,' _).
+    pose (i := is_var_get p); eassert (H : _) by exact (is_var_get_eq p); fold i in H |- *.
+    rewrite H; change (e ᵣ⊛ᵥ v_var x i) with ((e ᵣ⊛ v_var) x i).
+    unfold e_ren; rewrite v_sub_var; reflexivity.
+  Defined.
+
+  Variant is_var_ren_view {Γ1 Γ2 x} (v : val Γ1 x) (e : Γ1 ⊆ Γ2) : is_var (e ᵣ⊛ᵥ v) -> Type :=
+    | IsVarRen (p : is_var v) : is_var_ren_view v e (ren_is_var v e p)
+  .
+  Arguments IsVarRen {Γ1 Γ2 x v e}.
+
+  Lemma view_is_var_ren {Γ1 Γ2 x} (v : val Γ1 x) (e : Γ1 ⊆ Γ2) (p : is_var (e ᵣ⊛ᵥ v)) : is_var_ren_view v e p.
+    rewrite (is_var_irr p (ren_is_var v e (is_var_ren v e p))); econstructor.
+  Qed.
+
+
+(*|
+A couple derived properties on the constructed operations.
+|*)
+
+  #[global] Instance e_comp_proper {Γ1 Γ2 Γ3} :
+    Proper (ass_eq Γ2 Γ3 ==> ass_eq Γ1 Γ2 ==> ass_eq Γ1 Γ3) e_comp.
+  Proof.
+    intros ? ? H1 ? ? H2 ? i; unfold e_comp, s_map.
+    now rewrite H1, H2.
+  Qed.
+
+  #[global] Instance e_ren_proper {Γ1 Γ2 Γ3} :
+    Proper (ass_eq Γ2 Γ3 ==> ass_eq Γ1 Γ2 ==> ass_eq Γ1 Γ3) e_ren.
+  Proof.
+    intros ? ? H1 ? ? H2; unfold e_ren.
+    apply e_comp_proper; eauto; now rewrite H1.
+  Qed.
+
+  Lemma e_comp_ren_r {Γ1 Γ2 Γ3 Γ4} (u : Γ3 ⇒ᵥ Γ4) (v : Γ2 ⇒ᵥ Γ3) (w : Γ1 ⊆ Γ2)
+    : u ⊛ (v ⊛ᵣ w) ≡ₐ (u ⊛ v) ⊛ᵣ w.
+  Proof.
+    reflexivity.
+  Qed.
+
+  Lemma e_comp_ren_l {Γ1 Γ2 Γ3 Γ4} (u : Γ3 ⇒ᵥ Γ4) (v : Γ2 ⊆ Γ3) (w : Γ1 ⇒ᵥ Γ2)
+        : (u ⊛ᵣ v) ⊛ w ≡ₐ u ⊛ (v ᵣ⊛ w).
+  Proof.
+    unfold e_ren; now rewrite v_sub_sub, e_comp_ren_r, v_sub_var.
+  Qed.
+
+  Lemma v_sub_comp {Γ1 Γ2 Γ3} (u : Γ2 ⇒ᵥ Γ3) (v : Γ1 ⇒ᵥ Γ2) {x} (w : val Γ1 x) :
+    u ⊛ᵥ (v ⊛ᵥ w) = (u ⊛ v) ⊛ᵥ w.
+  Proof.
+    pose (w' := a_append a_empty w : (∅ ▶ x) ⇒ᵥ Γ1).
+    change w with (w' _ Ctx.top).
+    do 2 change (?u ⊛ᵥ ?v _ Ctx.top) with ((u ⊛ v) _ Ctx.top).
+    apply v_sub_sub.
+  Qed.
+
+  Lemma v_sub_id {Γ1 Γ2} (u : Γ1 ⇒ᵥ Γ2) {x} (i : Γ1 ∋ x) : u ⊛ᵥ (v_var x i) = u x i .
+    apply v_sub_var.
+  Qed.
+
+End withFam.
